Updates.

FOL/NV/Sub/Var/One/Ind/ReplaceFree.lean
@@ -10,82 +10,82 @@ open Formula_
 
 
 /--
-  IsReplaceFree F v t F' := True if and only if F' is the result of replacing in F each free occurrence of v by an occurrence of t.
+  is_replace_free_var_one F v t F' := True if and only if F' is the result of replacing in F each free occurrence of v by an occurrence of t.
 -/
-inductive IsReplaceFree : Formula_ → VarName_ → VarName_ → Formula_ → Prop
+inductive is_replace_free_var_one : Formula_ → VarName_ → VarName_ → Formula_ → Prop
 
   | pred_const_
     (X : PredName_)
     (xs : List VarName_)
     (v t : VarName_) :
-    IsReplaceFree (pred_const_ X xs) v t (pred_const_ X (xs.map fun (x : VarName_) =>
+    is_replace_free_var_one (pred_const_ X xs) v t (pred_const_ X (xs.map fun (x : VarName_) =>
       if v = x then t else x))
 
   | pred_var_
     (X : PredName_)
     (xs : List VarName_)
     (v t : VarName_) :
-    IsReplaceFree (pred_var_ X xs) v t (pred_var_ X (xs.map fun (x : VarName_) =>
+    is_replace_free_var_one (pred_var_ X xs) v t (pred_var_ X (xs.map fun (x : VarName_) =>
       if v = x then t else x))
 
   | eq_
     (x y : VarName_)
     (v t : VarName_) :
-    IsReplaceFree (eq_ x y) v t (eq_ (if v = x then t else x) (if v = y then t else y))
+    is_replace_free_var_one (eq_ x y) v t (eq_ (if v = x then t else x) (if v = y then t else y))
 
   | true_
     (v t : VarName_) :
-    IsReplaceFree true_ v t true_
+    is_replace_free_var_one true_ v t true_
 
   | false_
     (v t : VarName_) :
-    IsReplaceFree false_ v t false_
+    is_replace_free_var_one false_ v t false_
 
   | not_
     (phi : Formula_)
     (v t : VarName_)
     (phi' : Formula_) :
-    IsReplaceFree phi v t phi' →
-    IsReplaceFree phi.not_ v t phi'.not_
+    is_replace_free_var_one phi v t phi' →
+    is_replace_free_var_one phi.not_ v t phi'.not_
 
   | imp_
     (phi psi : Formula_)
     (v t : VarName_)
     (phi' psi' : Formula_) :
-    IsReplaceFree phi v t phi' →
-    IsReplaceFree psi v t psi' →
-    IsReplaceFree (phi.imp_ psi) v t (phi'.imp_ psi')
+    is_replace_free_var_one phi v t phi' →
+    is_replace_free_var_one psi v t psi' →
+    is_replace_free_var_one (phi.imp_ psi) v t (phi'.imp_ psi')
 
   | and_
     (phi psi : Formula_)
     (v t : VarName_)
     (phi' psi' : Formula_) :
-    IsReplaceFree phi v t phi' →
-    IsReplaceFree psi v t psi' →
-    IsReplaceFree (phi.and_ psi) v t (phi'.and_ psi')
+    is_replace_free_var_one phi v t phi' →
+    is_replace_free_var_one psi v t psi' →
+    is_replace_free_var_one (phi.and_ psi) v t (phi'.and_ psi')
 
   | or_
     (phi psi : Formula_)
     (v t : VarName_)
     (phi' psi' : Formula_) :
-    IsReplaceFree phi v t phi' →
-    IsReplaceFree psi v t psi' →
-    IsReplaceFree (phi.or_ psi) v t (phi'.or_ psi')
+    is_replace_free_var_one phi v t phi' →
+    is_replace_free_var_one psi v t psi' →
+    is_replace_free_var_one (phi.or_ psi) v t (phi'.or_ psi')
 
   | iff_
     (phi psi : Formula_)
     (v t : VarName_)
     (phi' psi' : Formula_) :
-    IsReplaceFree phi v t phi' →
-    IsReplaceFree psi v t psi' →
-    IsReplaceFree (phi.iff_ psi) v t (phi'.iff_ psi')
+    is_replace_free_var_one phi v t phi' →
+    is_replace_free_var_one psi v t psi' →
+    is_replace_free_var_one (phi.iff_ psi) v t (phi'.iff_ psi')
 
   | forall_not_free_in
     (x : VarName_)
     (phi : Formula_)
     (v t : VarName_) :
     v = x →
-    IsReplaceFree (forall_ x phi) v t (forall_ x phi)
+    is_replace_free_var_one (forall_ x phi) v t (forall_ x phi)
 
   | forall_free_in
     (x : VarName_)
@@ -93,15 +93,15 @@ inductive IsReplaceFree : Formula_ → VarName_ → VarName_ → Formula_ → Pr
     (v t : VarName_)
     (phi' : Formula_) :
     ¬ v = x →
-    IsReplaceFree phi v t phi' →
-    IsReplaceFree (forall_ x phi) v t (forall_ x phi')
+    is_replace_free_var_one phi v t phi' →
+    is_replace_free_var_one (forall_ x phi) v t (forall_ x phi')
 
   | exists_not_free_in
     (x : VarName_)
     (phi : Formula_)
     (v t : VarName_) :
     v = x →
-    IsReplaceFree (exists_ x phi) v t (exists_ x phi)
+    is_replace_free_var_one (exists_ x phi) v t (exists_ x phi)
 
   | exists_free_in
     (x : VarName_)
@@ -109,21 +109,21 @@ inductive IsReplaceFree : Formula_ → VarName_ → VarName_ → Formula_ → Pr
     (v t : VarName_)
     (phi' : Formula_) :
     ¬ v = x →
-    IsReplaceFree phi v t phi' →
-    IsReplaceFree (exists_ x phi) v t (exists_ x phi')
+    is_replace_free_var_one phi v t phi' →
+    is_replace_free_var_one (exists_ x phi) v t (exists_ x phi')
 
   | def_
     (X : DefName_)
     (xs : List VarName_)
     (v t : VarName_) :
-    IsReplaceFree (def_ X xs) v t (def_ X (xs.map fun (x : VarName_) =>
+    is_replace_free_var_one (def_ X xs) v t (def_ X (xs.map fun (x : VarName_) =>
       if v = x then t else x))
 
 
 example
   (F F' : Formula_)
   (v t : VarName_)
-  (h1 : IsReplaceFree F v t F') :
+  (h1 : is_replace_free_var_one F v t F') :
   Rec.fast_replace_free_var_one v t F = F' :=
   by
   induction h1
@@ -157,7 +157,7 @@ example
   (F F' : Formula_)
   (v t : VarName_)
   (h1 : Rec.fast_replace_free_var_one v t F = F') :
-  IsReplaceFree F v t F' :=
+  is_replace_free_var_one F v t F' :=
   by
   subst h1
   induction F
@@ -171,14 +171,14 @@ example
     | false_
     | def_ X xs =>
     first
-    | apply IsReplaceFree.pred_const_
-    | apply IsReplaceFree.pred_var_
-    | apply IsReplaceFree.eq_
-    | apply IsReplaceFree.true_
-    | apply IsReplaceFree.false_
-    | apply IsReplaceFree.def_
+    | apply is_replace_free_var_one.pred_const_
+    | apply is_replace_free_var_one.pred_var_
+    | apply is_replace_free_var_one.eq_
+    | apply is_replace_free_var_one.true_
+    | apply is_replace_free_var_one.false_
+    | apply is_replace_free_var_one.def_
   case not_ phi phi_ih =>
-    apply IsReplaceFree.not_
+    apply is_replace_free_var_one.not_
     exact phi_ih
   case
     imp_ phi psi phi_ih psi_ih
@@ -186,28 +186,28 @@ example
   | or_ phi psi phi_ih psi_ih
   | iff_ phi psi phi_ih psi_ih =>
     first
-    | apply IsReplaceFree.imp_
-    | apply IsReplaceFree.and_
-    | apply IsReplaceFree.or_
-    | apply IsReplaceFree.iff_
+    | apply is_replace_free_var_one.imp_
+    | apply is_replace_free_var_one.and_
+    | apply is_replace_free_var_one.or_
+    | apply is_replace_free_var_one.iff_
     · exact phi_ih
     · exact psi_ih
   case forall_ x phi phi_ih =>
     split_ifs
     case _ c1 =>
-      apply IsReplaceFree.forall_not_free_in
+      apply is_replace_free_var_one.forall_not_free_in
       exact c1
     case _ c1 =>
-      apply IsReplaceFree.forall_free_in
+      apply is_replace_free_var_one.forall_free_in
       · exact c1
       · exact phi_ih
   case exists_ x phi phi_ih =>
     split_ifs
     case _ c1 =>
-      apply IsReplaceFree.exists_not_free_in
+      apply is_replace_free_var_one.exists_not_free_in
       exact c1
     case _ c1 =>
-      apply IsReplaceFree.exists_free_in
+      apply is_replace_free_var_one.exists_free_in
       · exact c1
       · exact phi_ih
 
